theories/rules/send.v
@@ -1,14 +1,14 @@
 From machine_program_logic.program_logic Require Import weakestpre.
 From HypVeri Require Import lifting rules.rules_base stdpp_extra.
-From HypVeri.algebra Require Import base reg mem pagetable mailbox.
+From HypVeri.algebra Require Import base reg mem pagetable mailbox token.
 From HypVeri.lang Require Import lang_extra mem_extra reg_extra current_extra.
 Require Import stdpp.fin.
 
 Section send.
 
   Context `{vmG: !gen_VMG Σ}.
- (* TODO we forgot passing the control to vm0 *)
-Lemma hvc_send {wi r0 w sacc pi i j des ptx rxp l ai} :
+
+Lemma hvc_send_primary {wi r0 w sacc pi i j des ptx rxp l ai} :
   decode_instruction wi = Some(Hvc) ->
   addr_in_page ai pi ->
   decode_hvc_func r0 = Some(Send) ->
@@ -16,17 +16,18 @@ Lemma hvc_send {wi r0 w sacc pi i j des ptx rxp l ai} :
   pi ∈ sacc ->
   (finz.to_z l) = (Z.of_nat (length des)) ->
   ((length des) < page_size)%Z ->
+  fin_to_nat i = 0 -> 
   {SS{{ ▷(PC @@ i ->r ai) ∗ ▷ ai ->a wi ∗ ▷ A@i:={1}[sacc]
   ∗ ▷ (R0 @@ i ->r r0) ∗ ▷ (R1 @@ i ->r w) ∗ ▷ (R2 @@ i ->r l)
   ∗ ▷ TX@ i := ptx ∗ ▷ mem_region des ptx ∗ ▷ RX@ j :=( rxp !)
   ∗ ▷ (∃l', mem_region l' rxp ∗ ⌜length l' = length des⌝)}}}
    ExecI @ i {{{ RET ExecI ; PC @@ i ->r (ai ^+ 1)%f ∗ ai ->a wi
-  ∗ A@i:={1}[(sacc)]
-  ∗ R0 @@ i ->r (encode_hvc_ret_code Succ) ∗ R1 @@ i ->r w ∗ R2 @@ i ->r l
+  ∗ A@i:={1}[(sacc)] 
+  ∗ R0 @@ i ->r r0 ∗ R1 @@ i ->r w ∗ R2 @@ i ->r l
   ∗ TX@ i := ptx ∗ RX@ j :=( rxp ! l, i)
   ∗ mem_region des ptx ∗ mem_region des rxp }}}.
 Proof.
-  iIntros (Hdecodei Hinpi Hdecodef Hdecvmid Hpiacc Hlenl Hsize Φ).
+  iIntros (Hdecodei Hinpi Hdecodef Hdecvmid Hpiacc Hlenl Hsize Hz Φ).
   iIntros "(>PC & >Hai & >HA & >Hr0 & >Hr1 & >Hr2 & >HTX & >Hmemr & >HRX & >Hmemr') HΦ".
   iDestruct "Hmemr'" as "[%l' [Hmemr' %Hlen']]".
   iApply (sswp_lift_atomic_step ExecI); [done|].
@@ -61,7 +62,12 @@ Proof.
     iIntros (m2 σ2) "%HstepP".
     apply (step_ExecI_normal i Hvc ai wi) in HstepP; eauto.
     remember (exec Hvc σ1) as c2 eqn:Heqc2.
-    rewrite /exec /hvc HR0 Hdecodef /send HR1 /= Hdecvmid /= HR2 /= /transfer_msg /transfer_msg_unsafe in Heqc2.
+    assert (Hzeq : i = nat_to_fin vm_count_pos).
+    {
+      apply fin_to_nat_inj.
+      rewrite fin_to_nat_to_fin; auto.
+    }
+    rewrite /exec /hvc HR0 Hdecodef /send HR1 -Hzeq /= Hdecvmid /= HR2 /= /transfer_msg /transfer_msg_unsafe in Heqc2.
     assert (Hlendesclt :((Z.of_nat (length des)) <= (page_size-1))%Z).
     {
       apply (finz_plus_Z_le (of_pid ptx)); eauto.
@@ -79,6 +85,26 @@ Proof.
     destruct (get_vm_mail_box σ1 j) as [? [? rx]].
     simpl in Hrx2.
     rewrite Hrx2 /= in Heqc2.
+    rewrite /is_primary /= in Heqc2.
+    rewrite fill_rx_unsafe_preserve_current_vm copy_page_segment_unsafe_preserve_current_vm Hcureq Hz in Heqc2.
+    destruct (0 =? 0) eqn:Hvmz; [|done].
+    rewrite /= in Heqc2.
+    rewrite -Hcureq in Heqc2.
+    assert (Htemp : forall σ σ', (get_current_vm σ) = (get_current_vm σ') ->
+                                 update_current_vmid σ (get_current_vm σ') = σ).
+    intros σ σ' H.
+    rewrite -H /update_current_vmid
+            /get_reg_files /get_mail_boxes
+            /get_page_tables /get_current_vm
+            /get_mem /get_transactions.
+    by rewrite -!surjective_pairing.
+    rewrite Htemp in Heqc2; clear Htemp.
+    2 : {
+      rewrite /update_incr_PC /update_reg.
+      rewrite_reg_pc.
+      rewrite_reg_global.
+      by rewrite fill_rx_unsafe_preserve_current_vm copy_page_segment_unsafe_preserve_current_vm.
+    }
     destruct HstepP; subst m2 σ2; subst c2; simpl.
     rewrite /gen_vm_interp /update_incr_PC /update_reg.
     rewrite_reg_pc.
@@ -107,19 +133,12 @@ Proof.
     (* update regs *)
     rewrite -> (update_offset_PC_update_PC1 _ i ai 1); eauto.
     2 : {
-      rewrite !update_reg_global_update_reg fill_rx_unsafe_preserve_regs copy_page_segment_unsafe_preserve_regs;
-      try solve_reg_lookup.
-      rewrite !lookup_insert_ne; [|done].
-      rewrite get_reg_gmap_get_reg_Some; auto.
-    }
-    rewrite update_reg_global_update_reg.
-    2 : {
       rewrite fill_rx_unsafe_preserve_regs copy_page_segment_unsafe_preserve_regs;
       try solve_reg_lookup.
     }
-    iDestruct ((gen_reg_update2_global PC i _ (ai ^+ 1)%f R0 i _ (encode_hvc_ret_code Succ)) with "Hσreg PC Hr0") as ">[Hσreg [PC Hr0]]"; eauto.
+    iDestruct ((gen_reg_update1_global PC i _ (ai ^+ 1)%f) with "Hσreg PC") as ">[Hσreg PC]"; eauto.
     rewrite fill_rx_unsafe_preserve_regs copy_page_segment_unsafe_preserve_regs.
-    rewrite Hcureq.
+    rewrite Hcureq.    
     iFrame "Hσreg".
     (* update rx *)
     rewrite fill_rx_unsafe_update_mailbox.
@@ -214,6 +233,300 @@ Proof.
     split; auto.
     iApply "HΦ".
     rewrite Hlen'.
+    by iFrame.
+Qed.
+
+Lemma hvc_send_secondary {wi r0 w sacc pi i j des ptx rxp l ai z a b c} :
+  decode_instruction wi = Some(Hvc) ->
+  addr_in_page ai pi ->
+  decode_hvc_func r0 = Some(Send) ->
+  decode_vmid w = Some j ->
+  pi ∈ sacc ->
+  (finz.to_z l) = (Z.of_nat (length des)) ->
+  ((length des) < page_size)%Z ->
+  fin_to_nat z = 0 ->
+  i ≠ z ->
+  {SS{{ ▷(PC @@ i ->r ai) ∗ ▷ ai ->a wi ∗ ▷ A@i:={1}[sacc] ∗ ▷ (<<i>>{ 1%Qp })
+  ∗ ▷ (R0 @@ i ->r r0) ∗ ▷ (R1 @@ i ->r w) ∗ ▷ (R2 @@ i ->r l)
+  ∗ ▷ (R0 @@ z ->r a) ∗ ▷ (R1 @@ z ->r b) ∗ ▷ (R2 @@ z ->r c)
+  ∗ ▷ TX@ i := ptx ∗ ▷ mem_region des ptx ∗ ▷ RX@ j :=( rxp !)
+  ∗ ▷ (∃l', mem_region l' rxp ∗ ⌜length l' = length des⌝)}}}
+   ExecI @ i {{{ RET ExecI ; PC @@ i ->r (ai ^+ 1)%f ∗ ai ->a wi
+  ∗ A@i:={1}[(sacc)] ∗ <<z>>{ 1%Qp }
+  ∗ R0 @@ i ->r r0 ∗ R1 @@ i ->r w ∗ R2 @@ i ->r l
+  ∗ R0 @@ z ->r (encode_hvc_func Send) ∗ R1 @@ z ->r w ∗ R2 @@ z ->r l                     
+  ∗ TX@ i := ptx ∗ RX@ j :=( rxp ! l, i)
+  ∗ mem_region des ptx ∗ mem_region des rxp }}}.
+Proof.
+  iIntros (Hdecodei Hinpi Hdecodef Hdecvmid Hpiacc Hlenl Hsize Hz Hzine Φ).
+  iIntros "(>PC & >Hai & >HA & >Htoki & >Hr0 & >Hr1 & >Hr2 & >Hr0' & >Hr1' & >Hr2' & >HTX & >Hmemr & >HRX & >Hmemr') HΦ".
+  iDestruct "Hmemr'" as "[%l' [Hmemr' %Hlen']]".
+  iApply (sswp_lift_atomic_step ExecI); [done|].
+  iIntros (σ1) "%Hsche Hσ".
+  inversion Hsche as [Hcureq]; clear Hsche.
+  apply fin_to_nat_inj in Hcureq.
+  iModIntro.
+  iDestruct "Hσ" as "(Hcur & Hσmem & Hσreg & Hσtx & Hσrx1 & Hσrx2 & Hσowned & Hσaccess & Hσexcl & Htrans & Hσhp & %Hdisj & %Hlen & Hrcv)".
+  iDestruct ((gen_reg_valid4 i PC ai R0 r0 R1 w R2 l Hcureq) with "Hσreg PC Hr0 Hr1 Hr2")
+    as "[%HPC [%HR0 [%HR1 %HR2]]]"; eauto.
+  iDestruct ((gen_reg_valid_global1 R0 z a) with "Hσreg Hr0'") as %HR0'.
+  iDestruct ((gen_reg_valid_global1 R1 z b) with "Hσreg Hr1'") as %HR1'.
+  iDestruct ((gen_reg_valid_global1 R2 z c) with "Hσreg Hr2'") as %HR2'.
+  iDestruct ((gen_access_valid_addr_elem ai sacc) with "Hσaccess HA") as %Haccai; eauto.
+  { rewrite (to_pid_aligned_in_page _ pi); eauto. }
+  iDestruct ((gen_access_valid_pure sacc) with "Hσaccess HA") as %Hacc; eauto.
+  iDestruct (gen_mem_valid ai wi with "Hσmem Hai") as %Hai.
+  iDestruct (gen_mem_valid_SepL_pure _ des with "Hσmem Hmemr") as %Hadesc.
+  {
+    apply finz_seq_NoDup.
+    pose proof last_addr_in_bound as Hlaib.
+    specialize (Hlaib ptx).
+    solve_finz.
+  }
+  iDestruct (gen_tx_valid with "HTX Hσtx") as %Htx.
+  iDestruct (gen_rx_valid_none with "HRX Hσrx2") as %Hrx2.
+  iDestruct "HRX" as "(HRX1 & HRX2)".
+  iDestruct (gen_rx_pid_valid with "HRX1 Hσrx1") as %Hrx1.
+  iSplit.
+  - (* reducible *)
+    iPureIntro.
+    apply (reducible_normal i Hvc ai wi); eauto.
+  - (* step *)
+    iModIntro.
+    iIntros (m2 σ2) "%HstepP".
+    apply (step_ExecI_normal i Hvc ai wi) in HstepP; eauto.
+    remember (exec Hvc σ1) as c2 eqn:Heqc2.
+    assert (Hzeq : z = nat_to_fin vm_count_pos).
+    {
+      apply fin_to_nat_inj.
+      rewrite fin_to_nat_to_fin; auto.
+    }
+    rewrite /exec /hvc HR0 Hdecodef /send HR1 -Hzeq /= Hdecvmid /= HR2 /= /transfer_msg /transfer_msg_unsafe in Heqc2.
+    assert (Hlendesclt :((Z.of_nat (length des)) <= (page_size-1))%Z).
+    {
+      apply (finz_plus_Z_le (of_pid ptx)); eauto.
+      pose proof last_addr_in_bound as Hlaib.
+      specialize (Hlaib ptx).
+      solve_finz.
+      apply last_addr_in_bound.
+      solve_finz.
+    }
+    destruct (page_size <? l)%Z eqn:Hr1ps; [lia|].
+    rewrite /get_tx_pid_global Hcureq Htx /get_rx_pid_global /fill_rx Hrx1 in Heqc2.
+    assert (Hpreserve : get_vm_mail_box (copy_page_segment_unsafe σ1 ptx rxp l) j = get_vm_mail_box σ1 j).
+    f_equal.
+    rewrite Hpreserve in Heqc2.
+    destruct (get_vm_mail_box σ1 j) as [? [? rx]].
+    simpl in Hrx2.
+    rewrite Hrx2 /= in Heqc2.
+    rewrite /is_primary /= in Heqc2.
+    rewrite fill_rx_unsafe_preserve_current_vm copy_page_segment_unsafe_preserve_current_vm Hcureq in Heqc2.
+    destruct (i =? 0) eqn:Hi0.
+    rewrite <-(reflect_iff (fin_to_nat i = 0) (i =? 0) (Nat.eqb_spec (fin_to_nat i) 0)) in Hi0.
+    exfalso.
+    apply Hzine.
+    apply fin_to_nat_inj.
+    rewrite Hz Hi0.
+    reflexivity.
+    rewrite /= in Heqc2.
+    rewrite -Hcureq in Heqc2.
+    destruct HstepP; subst m2 σ2; subst c2; simpl.
+    rewrite /gen_vm_interp /update_incr_PC /update_reg.
+    rewrite_vmid_all.
+    rewrite_reg_pc.
+    do 3 rewrite_reg_global.
+    rewrite fill_rx_unsafe_preserve_mem
+            fill_rx_unsafe_preserve_rx1.
+    2 : {
+      rewrite /get_rx_pid_global Hpreserve.
+      reflexivity.
+    }
+    rewrite fill_rx_unsafe_preserve_tx.
+    2 : {
+      rewrite /get_tx_pid_global Hpreserve.
+      reflexivity.
+    }
+    rewrite fill_rx_unsafe_preserve_owned.
+    rewrite fill_rx_unsafe_preserve_access fill_rx_unsafe_preserve_excl.
+    rewrite fill_rx_unsafe_preserve_trans fill_rx_unsafe_preserve_hpool
+            fill_rx_unsafe_preserve_receivers.
+    rewrite copy_page_segment_unsafe_preserve_tx
+            copy_page_segment_unsafe_preserve_rx1 copy_page_segment_unsafe_preserve_owned
+            copy_page_segment_unsafe_preserve_access copy_page_segment_unsafe_preserve_excl
+            copy_page_segment_unsafe_preserve_trans copy_page_segment_unsafe_preserve_hpool
+            copy_page_segment_unsafe_preserve_receivers.
+    iFrame "Hσtx Hσrx1 Hσowned Hσaccess Hσexcl Htrans Hσhp Hrcv".
+    iEval (rewrite -Hcureq) in "Htoki".
+    iDestruct (token_update (get_current_vm σ1) (get_current_vm σ1) z with "Htoki") as "HtokUpd".
+    iDestruct ("HtokUpd" with "Hcur") as ">[Htokz Hcur]". 
+    rewrite /get_current_vm /update_current_vmid.
+    simpl.
+    iFrame "Hcur".
+    (* update regs *)
+    rewrite -> (update_offset_PC_update_PC1 _ i ai 1); eauto.
+    2 : {
+      rewrite get_reg_gmap_get_reg_Some; auto.
+      rewrite /get_reg //=.
+      do 3 rewrite_reg_global.
+      rewrite fill_rx_unsafe_preserve_current_vm copy_page_segment_unsafe_preserve_current_vm.
+      assert (Htemp : z ≠ get_current_vm σ1).
+      {
+        rewrite Hcureq.
+        intros Hcontra.
+        apply Hzine.
+        symmetry; auto.
+      }
+      do 3 (apply get_reg_global_update_reg_global_ne_vmid; auto).
+    }
+    rewrite update_reg_global_update_reg.
+    2 : {
+      exists c.
+      rewrite update_reg_global_update_reg.
+      rewrite lookup_insert_ne; auto.
+      rewrite update_reg_global_update_reg.
+      rewrite lookup_insert_ne; auto.
+      rewrite fill_rx_unsafe_preserve_regs copy_page_segment_unsafe_preserve_regs.
+      rewrite get_reg_gmap_lookup_Some.
+      rewrite /get_reg_global in HR2'.
+      assumption.
+      exists a.
+      rewrite fill_rx_unsafe_preserve_regs copy_page_segment_unsafe_preserve_regs.
+      rewrite get_reg_gmap_lookup_Some.
+      rewrite /get_reg_global in HR0'.
+      assumption.
+      exists b.
+      rewrite update_reg_global_update_reg.
+      rewrite lookup_insert_ne; auto.
+      rewrite fill_rx_unsafe_preserve_regs copy_page_segment_unsafe_preserve_regs.
+      rewrite get_reg_gmap_lookup_Some.
+      rewrite /get_reg_global in HR0'.
+      assumption.
+      exists a.
+      rewrite fill_rx_unsafe_preserve_regs copy_page_segment_unsafe_preserve_regs.
+      rewrite get_reg_gmap_lookup_Some.
+      rewrite /get_reg_global in HR0'.
+      assumption.
+    }
+    rewrite update_reg_global_update_reg.
+    2 : {
+      exists b.
+      rewrite update_reg_global_update_reg.
+      rewrite lookup_insert_ne; auto.
+      rewrite fill_rx_unsafe_preserve_regs copy_page_segment_unsafe_preserve_regs.
+      rewrite get_reg_gmap_lookup_Some.
+      rewrite /get_reg_global in HR0'.
+      assumption.
+      exists a.
+      rewrite fill_rx_unsafe_preserve_regs copy_page_segment_unsafe_preserve_regs.
+      rewrite get_reg_gmap_lookup_Some.
+      rewrite /get_reg_global in HR0'.
+      assumption.
+    }
+    rewrite update_reg_global_update_reg.
+    2 : {
+      exists a.
+      rewrite fill_rx_unsafe_preserve_regs copy_page_segment_unsafe_preserve_regs.
+      rewrite get_reg_gmap_lookup_Some.
+      rewrite /get_reg_global in HR0'.
+      assumption.
+    }
+    iDestruct ((gen_reg_update4_global PC i (ai ^+ 1)%f R2 z l R1 z w R0 z (encode_hvc_func Send)) with "Hσreg PC Hr2' Hr1' Hr0'") as ">[Hσreg [PC [Hr2' [Hr1' Hr0']]]]"; eauto.
+    rewrite fill_rx_unsafe_preserve_regs copy_page_segment_unsafe_preserve_regs.    
+    iFrame "Hσreg".
+    (* update rx *)
+    rewrite fill_rx_unsafe_update_mailbox.
+    rewrite copy_page_segment_unsafe_preserve_rx2.
+    iCombine "HRX1 HRX2" as "HRX". 
+    iDestruct ((gen_rx_gmap_update_global_None j l (get_current_vm σ1) rxp) with "Hσrx2 HRX") as ">[Hσrx' [HRX1 HRX2]]".
+    iEval (rewrite /get_current_vm) in "Hσrx'".
+    iFrame "Hσrx'".
+    (* update mem *)
+    rewrite /copy_page_segment_unsafe /copy_from_addr_to_addr_unsafe //=.
+    assert (Hlist: read_mem_segment_unsafe σ1 ptx l = des).
+    {
+      rewrite /read_mem_segment_unsafe.
+      rewrite /get_mem in Hadesc.
+      apply (f_equal Z.to_nat) in Hlenl.
+      rewrite Hlenl.
+      rewrite Nat2Z.id.
+      clear Hlenl Hlendesclt Htx Hpreserve Hlen' Hsize.
+      generalize dependent (of_pid ptx).
+      induction des; first done.
+      simpl in IHdes.
+      simpl.
+      intros.
+      rewrite /get_memory_unsafe.
+      rewrite (Hadesc 0 f a0).
+      simpl.
+      f_equal.
+      rewrite /get_memory_unsafe in IHdes.
+      rewrite (IHdes (f ^+ 1)%f).
+      reflexivity.
+      intros k y1 y2 H1 H2.
+      apply Hadesc with (S k); auto.
+      reflexivity.
+      reflexivity.
+    }
+    rewrite Hlist.
+    rewrite /write_mem_segment_unsafe //.
+    iDestruct ((gen_mem_update_SepL2 (finz.seq rxp (length l')) l' des) with "Hσmem Hmemr'") as "Hmemupd".
+    rewrite Hlen'.
+    apply finz_seq_NoDup'.
+    pose proof last_addr_in_bound as Hbound.
+    specialize (Hbound rxp).
+    solve_finz.
+    assumption.
+    (* TODO make a general lemma in lang_extra *)
+    assert (Hzipeq : (zip (finz.seq rxp (length l')) des) = (zip (finz.seq rxp (Z.to_nat 1000)) des)).
+    {
+      rewrite <-(zip_fst_snd (zip (finz.seq rxp (Z.to_nat 1000)) des)).
+      rewrite !snd_zip; auto.
+      f_equal.
+      rewrite Hlen'.
+      clear Hlenl Hadesc Hlist Hlen' Hsize.
+      generalize dependent (of_pid rxp).
+      induction des; first done.
+      cbn.
+      destruct (Z.to_nat 1000) eqn:Heqn1000; first done.
+      simpl.
+      intros f.
+      f_equal.
+      assert (Hn : n = 999).
+      lia.
+      subst n.
+      rewrite (@zip_length_le _ _ des (finz.seq (f ^+ 1)%f 999) (finz.seq (f ^+ 1)%f 1000) [(f ^+ 1000)%f]).
+      simpl in Hlendesclt.
+      rewrite IHdes.
+      reflexivity.
+      lia.
+      simpl in Hlendesclt.
+      rewrite finz_seq_length.
+      lia.
+      rewrite (finz_seq_decomposition _ 1000 _ 999).
+      f_equal.
+      simpl.
+      f_equal.
+      rewrite Unnamed_thm12.
+      rewrite Z.add_comm.
+      assert (H999_1 : Z.add (Z.of_nat 999%nat) 1%Z = 1000%Z).
+      reflexivity.
+      rewrite H999_1.
+      reflexivity.
+      lia.
+      lia.
+      lia.
+      rewrite finz_seq_length.
+      lia.
+    }
+    rewrite Hzipeq.
+    iDestruct "Hmemupd" as ">[Hmemupd1 Hmemupd2]".
+    iFrame "Hmemupd1".
+    iSplitR.
+    iPureIntro.
+    split; auto.
+    iApply "HΦ".
+    rewrite Hlen'.
+    rewrite -Hcureq.
     by iFrame.
 Qed.
 
